System, movers, and refinement for concur-tree

ironfleet/src/Dafny/Distributed/Concur/Refinement.i.dfy
@@ -1,59 +1,79 @@
-include "DistributedSystem.i.dfy"
+include "System.i.dfy"
 include "Movers.i.dfy"
 
 module RefinementModule {
 
-    import opened DistributedSystemModule
+    import opened SystemModule
     import opened MoversModule
 
     type SpecState
+    type SpecBehavior = seq<SpecState>
+    type SpecMultibehavior = seq<SpecBehavior>
     predicate SpecInit(ss:SpecState)
     predicate SpecNext(ss:SpecState, ss':SpecState)
-    predicate SpecCorrespondence(ds:DistributedSystemState, ss:SpecState)
+    predicate SpecCorrespondence(ds:SystemState, ss:SpecState)
 
-    lemma {:axiom} lemma_RightMoverForwardPreservation(rightMover:Entry, ds:DistributedSystemState, ds':DistributedSystemState, ss:SpecState)
+    lemma {:axiom} lemma_RightMoverForwardPreservation(rightMover:Entry, ds:SystemState, ds':SystemState, ss:SpecState)
         requires EntryIsRightMover(rightMover);
-        requires DistributedSystemNextEntryAction(ds, ds', rightMover);
+        requires SystemNextEntry(ds, ds', rightMover);
         requires SpecCorrespondence(ds, ss);
         ensures  SpecCorrespondence(ds', ss);
 
-    lemma {:axiom} lemma_LeftMoverBackwardPreservation(leftMover:Entry, ds:DistributedSystemState, ds':DistributedSystemState, ss:SpecState)
+    lemma {:axiom} lemma_LeftMoverBackwardPreservation(leftMover:Entry, ds:SystemState, ds':SystemState, ss:SpecState)
         requires EntryIsLeftMover(leftMover);
-        requires DistributedSystemNextEntryAction(ds, ds', leftMover);
+        requires SystemNextEntry(ds, ds', leftMover);
         requires SpecCorrespondence(ds', ss);
         ensures  SpecCorrespondence(ds, ss);
 
-    predicate IsValidSpecBehavior(sb:seq<SpecState>)
+    predicate SpecNextOrStutter(ss:SpecState, ss':SpecState)
+    {
+           SpecNext(ss, ss')
+        || ss == ss'
+    }
+        
+    predicate IsValidSpecBehavior(sb:SpecBehavior)
     {
            |sb| > 0
         && SpecInit(sb[0])
-        && (forall i :: 0 <= i < |sb| - 1 ==> (SpecNext(sb[i], sb[i+1]) || sb[i] == sb[i+1]))
+        && (forall i {:trigger SpecNextOrStutter(sb[i], sb[i+1])}{:trigger SpecNext(sb[i], sb[i+1])} ::
+                 0 <= i < |sb| - 1 ==> SpecNextOrStutter(sb[i], sb[i+1]))
     }
 
-    predicate IsValidDistributedSystemBehavior(db:seq<DistributedSystemState>)
+    function ConcatenationOfSpecMultibehavior(sm:SpecMultibehavior) : SpecBehavior
+    {
+        if |sm| == 0 then [] else sm[0] + ConcatenationOfSpecMultibehavior(sm[1..])
+    }
+
+    predicate IsValidSpecMultibehavior(sm:SpecMultibehavior)
+    {
+           IsValidSpecBehavior(ConcatenationOfSpecMultibehavior(sm))
+        && (forall b :: b in sm ==> |b| > 0)
+    }
+
+    predicate IsValidSystemBehavior(db:SystemBehavior)
     {
            |db| > 0
-        && DistributedSystemInit(db[0])
-        && (forall i :: 0 <= i < |db| - 1 ==> DistributedSystemNext(db[i], db[i+1]))
+        && SystemInit(db[0])
+        && (forall i {:trigger SystemNext(db[i], db[i+1])} :: 0 <= i < |db| - 1 ==> SystemNext(db[i], db[i+1]))
     }
 
-    predicate IsValidDistributedSystemTraceAndBehavior(trace:Trace, db:seq<DistributedSystemState>)
+    predicate IsValidSystemTraceAndBehavior(trace:Trace, db:SystemBehavior)
     {
            |db| == |trace| + 1
-        && DistributedSystemInit(db[0])
-        && (forall i :: 0 <= i < |trace| ==> DistributedSystemNextEntryAction(db[i], db[i+1], trace[i]))
+        && SystemInit(db[0])
+        && (forall i {:trigger SystemNextEntry(db[i], db[i+1], trace[i])} :: 0 <= i < |trace| ==> SystemNextEntry(db[i], db[i+1], trace[i]))
     }
 
-    predicate DistributedSystemBehaviorRefinesSpecBehavior(db:seq<DistributedSystemState>, sb:seq<SpecState>)
+    predicate SystemBehaviorRefinesSpecMultibehavior(db:SystemBehavior, sm:SpecMultibehavior)
     {
-           |db| == |sb|
-        && IsValidSpecBehavior(sb)
-        && (forall i :: 0 <= i < |db| ==> SpecCorrespondence(db[i], sb[i]))
+           |db| == |sm|
+        && IsValidSpecMultibehavior(sm)
+        && (forall i, ss {:trigger SpecCorrespondence(db[i], ss)} :: 0 <= i < |db| && ss in sm[i] ==> SpecCorrespondence(db[i], ss))
     }
 
-    predicate DistributedSystemBehaviorRefinesSpec(db:seq<DistributedSystemState>)
+    predicate SystemBehaviorRefinesSpec(db:SystemBehavior)
     {
-        exists sb :: DistributedSystemBehaviorRefinesSpecBehavior(db, sb)
+        exists sm :: SystemBehaviorRefinesSpecMultibehavior(db, sm)
     }
 
 }
