ironfleet/src/Dafny/Distributed/Concur/Movers.i.dfy
@@ -1,187 +1,53 @@
-include "DistributedSystem.i.dfy"
+include "System.i.dfy"
 
 module MoversModule {
 
-    import opened DistributedSystemModule
-
-    predicate IOActionIsRightMover(io:IOAction)
-    {
-        io.IOActionReceive? || io.IOActionUpdateLocalState? || io.IOActionStutter?
-    }
-
-    predicate IOActionIsLeftMover(io:IOAction)
-    {
-        io.IOActionSend? || io.IOActionUpdateLocalState? || io.IOActionStutter?
-    }
+    import opened SystemModule
 
     predicate ActionIsRightMover(action:Action)
     {
-        action.ActionIO? && IOActionIsRightMover(action.io)
+        action.Receive? || action.UpdateLocalState? || action.Stutter?
     }
 
     predicate ActionIsLeftMover(action:Action)
     {
-        action.ActionIO? && IOActionIsLeftMover(action.io)
+        action.Send? || action.UpdateLocalState? || action.Stutter?
     }
 
     predicate EntryIsRightMover(entry:Entry)
     {
-        entry.EntryAction? ==> ActionIsRightMover(entry.action)
+        ActionIsRightMover(entry.action)
     }
 
     predicate EntryIsLeftMover(entry:Entry)
     {
-        entry.EntryAction? ==> ActionIsLeftMover(entry.action)
+        ActionIsLeftMover(entry.action)
     }
 
-    lemma lemma_MoverCommutativityForIOActions(
-        actor1:Actor,
-        actor2:Actor,
-        io1:IOAction,
-        io2:IOAction,
-        ds1:DistributedSystemState,
-        ds2:DistributedSystemState,
-        ds3:DistributedSystemState
-        )
-        returns
-        (ds2':DistributedSystemState)
-        requires actor1 != actor2;
-        requires DistributedSystemNextIOAction(ds1, ds2, actor1, io1);
-        requires DistributedSystemNextIOAction(ds2, ds3, actor2, io2);
-        requires IOActionIsRightMover(io1) || IOActionIsLeftMover(io2);
-        ensures  DistributedSystemNextIOAction(ds1, ds2', actor2, io2);
-        ensures  DistributedSystemNextIOAction(ds2', ds3, actor1, io1);
-    {
-        if io1.IOActionReceive? {
-            ds2' := ds3;
-        }
-        else if io1.IOActionUpdateLocalState? {
-            if actor1 in ds1.states {
-                ds2' := ds3.(states := ds3.states[actor1 := ds1.states[actor1]]);
-                if !io2.IOActionUpdateLocalState? {
-                    assert ds2'.states == ds1.states;
-                }
-            }
-            else {
-                assert ds1.states == ds2.states;
-                ds2' := ds3;
-            }
-        }
-        else if io1.IOActionStutter? {
-            ds2' := ds3;
-        }
-        else if io2.IOActionStutter? {
-            ds2' := ds1;
-        }
-        else if io2.IOActionUpdateLocalState? {
-            if actor2 in ds2.states {
-                ds2' := ds1.(states := ds3.states);
-            }
-            else {
-                ds2' := ds1;
-                assert ds2.states == ds3.states;
-            }
-        }
-        else if io2.IOActionSend? {
-            ds2' := ds1.(sentPackets := ds1.sentPackets + {io2.s});
-            if io1.IOActionSend? {
-                assert ds3.sentPackets == ds2'.sentPackets + {io1.s};
-            }
-        }
-    }
-
-    lemma lemma_MoverCommutativityForActions(
-        actor1:Actor,
-        actor2:Actor,
-        action1:Action,
-        action2:Action,
-        ds1:DistributedSystemState,
-        ds2:DistributedSystemState,
-        ds3:DistributedSystemState
-        )
-        returns
-        (ds2':DistributedSystemState)
-        requires actor1 != actor2;
-        requires DistributedSystemNextAction(ds1, ds2, actor1, action1);
-        requires DistributedSystemNextAction(ds2, ds3, actor2, action2);
-        requires ActionIsRightMover(action1) || ActionIsLeftMover(action2);
-        ensures  DistributedSystemNextAction(ds1, ds2', actor2, action2);
-        ensures  DistributedSystemNextAction(ds2', ds3, actor1, action1);
-    {
-        if action1.ActionIO? && action1.io.IOActionReceive? {
-            ds2' := ds3;
-        }
-        else if action1.ActionIO? && action1.io.IOActionUpdateLocalState? {
-            if actor1 in ds1.states {
-                ds2' := ds3.(states := ds3.states[actor1 := ds1.states[actor1]]);
-                if !(action2.ActionIO? && action2.io.IOActionUpdateLocalState?) &&
-                   !(action2.ActionDS? && action2.ds.DSActionHostEventHandler?) {
-                    assert ds2'.states == ds1.states;
-                }
-            }
-            else {
-                assert ds1.states == ds2.states;
-                ds2' := ds3;
-            }
-        }
-        else if action1.ActionIO? && action1.io.IOActionStutter? {
-            ds2' := ds3;
-        }
-        else if action2.ActionIO? && action2.io.IOActionStutter? {
-            ds2' := ds1;
-        }
-        else if action2.ActionIO? && action2.io.IOActionUpdateLocalState? {
-            if actor2 in ds2.states {
-                ds2' := ds1.(states := ds1.states[actor2 := ds3.states[actor2]]);
-                if !(action1.ActionIO? && action1.io.IOActionUpdateLocalState?) &&
-                   !(action1.ActionDS? && action1.ds.DSActionHostEventHandler?) {
-                    assert ds2'.states == ds3.states;
-                }
-            }
-            else {
-                ds2' := ds1;
-                assert ds2.states == ds3.states;
-            }
-        }
-        else if action2.ActionIO? && action2.io.IOActionSend? {
-            ds2' := ds1.(sentPackets := ds1.sentPackets + {action2.io.s});
-            if action1.ActionIO? && action1.io.IOActionSend? {
-                assert ds2'.states == ds3.states;
-                assert ds3.sentPackets == ds2'.sentPackets + {action1.io.s};
-            }
-            else if action1.ActionDS? && action1.ds.DSActionHostEventHandler? {
-                assert ds2'.states == ds1.states;
-            }
-        }
-    }
 
     lemma lemma_MoverCommutativityForEntries(
         entry1:Entry,
         entry2:Entry,
-        ds1:DistributedSystemState,
-        ds2:DistributedSystemState,
-        ds3:DistributedSystemState
+        ds1:SystemState,
+        ds2:SystemState,
+        ds3:SystemState
         )
         returns
-        (ds2':DistributedSystemState)
-        requires GetEntryActor(entry1) != GetEntryActor(entry2);
-        requires DistributedSystemNextEntryAction(ds1, ds2, entry1);
-        requires DistributedSystemNextEntryAction(ds2, ds3, entry2);
+        (ds2':SystemState)
+        requires entry1.actor != entry2.actor;
+        requires SystemNextEntry(ds1, ds2, entry1);
+        requires SystemNextEntry(ds2, ds3, entry2);
         requires EntryIsRightMover(entry1) || EntryIsLeftMover(entry2);
-        ensures  DistributedSystemNextEntryAction(ds1, ds2', entry2);
-        ensures  DistributedSystemNextEntryAction(ds2', ds3, entry1);
+        ensures  SystemNextEntry(ds1, ds2', entry2);
+        ensures  SystemNextEntry(ds2', ds3, entry1);
     {
-        if !entry1.EntryAction? {
+        if entry1.action.Receive? {
             ds2' := ds3;
         }
-        else if entry1.EntryAction? && entry1.action.ActionIO? && entry1.action.io.IOActionReceive? {
-            ds2' := ds3;
-        }
-        else if entry1.EntryAction? && entry1.action.ActionIO? && entry1.action.io.IOActionUpdateLocalState? {
+        else if entry1.action.UpdateLocalState? {
             if entry1.actor in ds1.states {
                 ds2' := ds3.(states := ds3.states[entry1.actor := ds1.states[entry1.actor]]);
-                if !(entry2.EntryAction? && entry2.action.ActionIO? && entry2.action.io.IOActionUpdateLocalState?) &&
-                   !(entry2.EntryAction? && entry2.action.ActionDS? && entry2.action.ds.DSActionHostEventHandler?) {
+                if !entry2.action.UpdateLocalState? && !entry2.action.PerformIos? && !entry2.action.HostNext? {
                     assert ds2'.states == ds1.states;
                 }
             }
@@ -190,20 +56,16 @@ module MoversModule {
                 ds2' := ds3;
             }
         }
-        else if entry1.EntryAction? && entry1.action.ActionIO? && entry1.action.io.IOActionStutter? {
+        else if entry1.action.Stutter? {
             ds2' := ds3;
         }
-        else if !entry2.EntryAction? {
+        else if entry2.action.Stutter? {
             ds2' := ds1;
         }
-        else if entry2.EntryAction? && entry2.action.ActionIO? && entry2.action.io.IOActionStutter? {
-            ds2' := ds1;
-        }
-        else if entry2.EntryAction? && entry2.action.ActionIO? && entry2.action.io.IOActionUpdateLocalState? {
+        else if entry2.action.UpdateLocalState? {
             if entry2.actor in ds2.states {
                 ds2' := ds1.(states := ds1.states[entry2.actor := ds3.states[entry2.actor]]);
-                if !(entry1.EntryAction? && entry1.action.ActionIO? && entry1.action.io.IOActionUpdateLocalState?) &&
-                   !(entry1.EntryAction? && entry1.action.ActionDS? && entry1.action.ds.DSActionHostEventHandler?) {
+                if !entry1.action.UpdateLocalState? && !entry1.action.PerformIos? && !entry1.action.HostNext? {
                     assert ds2'.states == ds3.states;
                 }
             }
@@ -212,13 +74,16 @@ module MoversModule {
                 assert ds2.states == ds3.states;
             }
         }
-        else if entry2.EntryAction? && entry2.action.ActionIO? && entry2.action.io.IOActionSend? {
-            ds2' := ds1.(sentPackets := ds1.sentPackets + {entry2.action.io.s});
-            if entry1.EntryAction? && entry1.action.ActionIO? && entry1.action.io.IOActionSend? {
+        else if entry2.action.Send? {
+            ds2' := ds1.(sentPackets := ds1.sentPackets + {entry2.action.s});
+            if entry1.action.Send? {
                 assert ds2'.states == ds3.states;
-                assert ds3.sentPackets == ds2'.sentPackets + {entry1.action.io.s};
+                assert ds3.sentPackets == ds2'.sentPackets + {entry1.action.s};
             }
-            else if entry1.EntryAction? && entry1.action.ActionDS? && entry1.action.ds.DSActionHostEventHandler? {
+            else if entry1.action.PerformIos? {
+                assert ds2'.states == ds1.states;
+            }
+            else if entry1.action.HostNext? {
                 assert ds2'.states == ds1.states;
             }
         }
