ironfleet/src/Dafny/Distributed/Concur/System.i.dfy
@@ -1,0 +1,129 @@
+include "Trace.i.dfy"
+
+module SystemModule {
+
+    import opened TraceModule
+
+    type ActorState
+    predicate ActorStateInit(s:ActorState)
+    predicate HostNext(s:ActorState, s':ActorState, ios:seq<Action>)
+
+    datatype SystemState = SystemState(states:map<Actor, ActorState>, time:int, sentPackets:set<Packet>)
+    type SystemBehavior = seq<SystemState>
+
+    predicate SystemInit(s:SystemState)
+    {
+           (forall actor :: actor in s.states ==> ActorStateInit(s.states[actor]))
+        && |s.sentPackets| == 0
+        && s.time >= 0
+    }
+
+    predicate SystemNextReceive(s:SystemState, s':SystemState, actor:Actor, p:Packet)
+    {
+           s' == s
+        && actor.HostActor?
+        && p in s.sentPackets
+        && p.dst == actor.ep
+    }
+
+    predicate SystemNextSend(s:SystemState, s':SystemState, actor:Actor, p:Packet)
+    {
+           s' == s.(sentPackets := s.sentPackets + {p})
+        && actor.HostActor?
+        && p.src == actor.ep
+    }
+
+    predicate SystemNextReadClock(s:SystemState, s':SystemState, actor:Actor, t:int)
+    {
+           s' == s
+        && actor.HostActor?
+        && t == s.time
+    }
+
+    predicate SystemNextUpdateLocalState(s:SystemState, s':SystemState, actor:Actor)
+    {
+           actor.HostActor?
+        && (forall any_actor :: any_actor in s.states <==> any_actor in s'.states)
+        && (forall other_actor :: other_actor != actor && other_actor in s.states ==>
+                            other_actor in s'.states && s'.states[other_actor] == s.states[other_actor])
+        && s'.sentPackets == s.sentPackets
+        && s'.time == s.time
+    }
+
+    predicate SystemNextStutter(s:SystemState, s':SystemState)
+    {
+        s' == s
+    }
+
+    predicate SystemNextDeliverPacket(s:SystemState, s':SystemState, p:Packet)
+    {
+           p in s.sentPackets
+        && s' == s
+    }
+
+    predicate SystemNextAdvanceTime(s:SystemState, s':SystemState, t:int)
+    {
+           t > s.time
+        && s' == s.(time := t)
+    }
+
+    predicate SystemNextPerformIos(
+        s:SystemState,
+        s':SystemState,
+        actor:Actor,
+        ios:seq<Action>
+        )
+    {
+           actor.HostActor?
+        && s'.states == s.states
+        && s'.time == s.time
+        && (forall p :: p in s.sentPackets ==> p in s'.sentPackets)
+        && (forall p :: p in s'.sentPackets ==> p in s.sentPackets || Send(p) in ios)
+        && (forall io :: io in ios && io.Receive? ==> io.r in s.sentPackets && io.r.dst == actor.ep)
+        && (forall io :: io in ios && io.Send? ==> io.s in s'.sentPackets && io.s.src == actor.ep)
+    }
+
+    predicate SystemNextHostNext(
+        s:SystemState,
+        s':SystemState,
+        actor:Actor,
+        ios:seq<Action>
+        )
+    {
+           actor.HostActor?
+        && actor in s.states
+        && actor in s'.states
+        && s'.states == s.states[actor := s'.states[actor]]
+        && HostNext(s.states[actor], s'.states[actor], ios)
+        && s'.time == s.time
+        && (forall p :: p in s.sentPackets ==> p in s'.sentPackets)
+        && (forall p :: p in s'.sentPackets ==> p in s.sentPackets || Send(p) in ios)
+        && (forall io :: io in ios && io.Receive? ==> io.r in s.sentPackets && io.r.dst == actor.ep)
+        && (forall io :: io in ios && io.Send? ==> io.s in s'.sentPackets && io.s.src == actor.ep)
+    }
+
+    predicate SystemNextAction(s:SystemState, s':SystemState, actor:Actor, action:Action)
+    {
+        match action
+            case Receive(p) => SystemNextReceive(s, s', actor, p)
+            case Send(p) => SystemNextSend(s, s', actor, p)
+            case ReadClock(t) => SystemNextReadClock(s, s', actor, t)
+            case UpdateLocalState => SystemNextUpdateLocalState(s, s', actor)
+            case Stutter => SystemNextStutter(s, s')
+            case DeliverPacket(p) => SystemNextDeliverPacket(s, s', p)
+            case AdvanceTime(t) => SystemNextAdvanceTime(s, s', t)
+            case PerformIos(ios) => SystemNextPerformIos(s, s', actor, ios)
+            case HostNext(ios) => SystemNextHostNext(s, s', actor, ios)
+    }
+
+    predicate SystemNextEntry(s:SystemState, s':SystemState, entry:Entry)
+    {
+        SystemNextAction(s, s', entry.actor, entry.action)
+    }
+
+    predicate SystemNext(s:SystemState, s':SystemState)
+    {
+        exists entry :: SystemNextEntry(s, s', entry)
+    }
+
+}
